Common.v
@@ -150,4 +150,13 @@ Section Security.
     | LevelP l => l
     | ErasureP l1 cnd l2 _ => if (set_mem Nat.eq_dec cnd U) then l1 else l2
     end.
+
+  Inductive protected : sec_policy -> set condition -> Prop :=
+  | level_high: forall S, protected (LevelP H) S
+  | level_top: forall S, protected (LevelP T) S
+  | erase_high: forall cnd S sl pf,
+      protected (ErasureP H cnd sl pf) S
+  | erase_low: forall cnd S sl pf,
+      set_In cnd S -> protected (ErasureP L cnd sl pf) S.
+
 End Security.
